\renewcommand{\theequation}{\theenumi}
\begin{enumerate}[label=\arabic*.,ref=\thesubsection.\theenumi]
\numberwithin{equation}{enumi}
\item


A right angled triangle looks like Fig. \ref{fig:tri_right_angle}.
\begin{figure}[!ht]
\centering
\resizebox{\columnwidth}{!}{\input{./figs/triangle/tri_right_angle.tex}}
\caption{Right Angled Triangle}
\label{fig:tri_right_angle}	
\end{figure}
with angles $\angle A,\angle B$ and $\angle C$ and sides $a, b$ and $c$.  The unique feature of this triangle is $\angle B$ which is defined to be $90\degree$.
\item
	For simplicity, let the greek letter $\theta = \angle C$.  We have the following definitions.
\begin{equation}
\label{eq:tri_trig_defs}
\begin{matrix}
	\sin \theta = \frac{c}{b} & 	\cos \theta = \frac{a}{b} \\
	\tan \theta = \frac{c}{a} & \cot \theta = \frac{1}{\tan \theta} \\
	\csc \theta = \frac{1}{\sin \theta} & \sec \theta = \frac{1}{\cos \theta}
	\end{matrix}
\end{equation}
%
\item Draw Fig. \ref{fig:tri_right_angle} for $a = 4, c =3$.
\label{const:tri_right_angle}
%
\\
\solution The vertices of $\triangle ABC$ are 
\begin{align}
\vec{A} = \myvec{0\\c} = \myvec{0\\3}, \vec{B} = \myvec{0\\0}, \vec{C} = \myvec{a\\0}=\myvec{4\\0}
\end{align}
%
The python code for  Fig. \ref{fig:tri_right_angle} is
\begin{lstlisting}
codes/triangle/tri_right_angle.py
\end{lstlisting}
%
and the equivalent latex-tikz code is
%
\begin{lstlisting}
figs/triangle/tri_right_angle.tex
\end{lstlisting}
%
\item Draw Fig. \ref{fig:tri_polar} for $a = 4, c =3$.
\label{const:tri_polar}
%
\\
\solution The vertices of $\triangle ABC$ are 
\begin{align}
\vec{A} = \myvec{a\\c} = \myvec{4\\3}, \vec{B} = \myvec{a\\0}  = \myvec{4\\0}, \vec{C} = \myvec{0\\0}.
\end{align}
%
The python code for  Fig. \ref{fig:tri_polar} is
\begin{lstlisting}
codes/triangle/tri_polar.py
\end{lstlisting}
%
and the equivalent latex-tikz code is
%
\begin{lstlisting}
figs/triangle/tri_polar.tex
\end{lstlisting}
\begin{figure}[!ht]
\centering
\resizebox{\columnwidth}{!}{\input{./figs/triangle/tri_polar.tex}}
\caption{Right Angled Triangle}
\label{fig:tri_polar}	
\end{figure}
%
\item The vertex  $\vec{A}$ can also be expressed  in {\em polar coordinate form} as
\label{prob:tri_polar}
%
\begin{align}
\vec{A} = \myvec{b\cos \theta\\ b \sin \theta} 
\end{align}
%

\end{enumerate}

%\subsection{Sum of Angles}
%\renewcommand{\theequation}{\theenumi}
%\begin{enumerate}[label=\arabic*.,ref=\thesubsection.\theenumi]
%\numberwithin{equation}{enumi}
%\item 	In Fig. \ref{fig:tri_sum_angle}, the sum of all the angles on the top or bottom side of the straight line $XY$ is $180\degree$.
%
%
%\begin{figure}[!ht]
%	\begin{center}
%		\resizebox{\columnwidth}{!}{\input{./figs/triangle/tri_sum_angle.tex}}
%	\end{center}
%	\caption{Sum of angles of a triangle}
%	\label{fig:tri_sum_angle}	
%\end{figure}
%
%
%
%\item
%In Fig. \ref{fig:tri_sum_angle}, the straight line making an angle of $90\degree$ to the side $AB$ is said to be parallel to the side $BC$. Note there is an angle at $A$ that is equal to $\theta$.  This is one property of parallel lines.  Thus, $\angle YAZ = 90\degree$.
%
%
%\item
%	Show that $\angle VAZ = 90\degree - \theta$
%		
%	\solution Considering the line $XAZ$,
%	\begin{align}
%	\theta + 90\degree + \angle VAZ &= 180\degree \\
%	\Rightarrow  \angle VAZ =  90\degree - \theta
%	\end{align}
%
%\item
%	\label{prob:tri_compl_angle}
%	Show that $\angle BAC = 90\degree - \theta$.
%	
%	\solution Consider the line $VAB$ and and use the approach in the previous problem.  Note that this implies that $\angle VAZ = \angle BAC$.  Such angles are known as vertically opposite angles. 
%	 
%\item
%Sum of the angles of a triangle is equal to $180\degree$.
%%
%\item Draw Fig. \ref{fig:tri_sum_angle} for $a = 4, c =3$.
%%
%\\
%\solution Problem \ref{const:tri_right_angle} is used to draw $\triangle ABC$.  The remaining points are obtained as
%
%\begin{align}
%\vec{Y} &= \vec{A} + \myvec{1\\0} = \myvec{1\\3}
%\\
%\vec{X} &= \vec{A} - \myvec{1\\0} = \myvec{-1\\3}
%\\
%\vec{T} &= \vec{A} + \myvec{0\\1} = \myvec{0\\4}
%\end{align}
%%
%and 
%\begin{align}
%\frac{VC}{AC} &= k+1
%\\
%\label{eq:tri_section_formula}
%\implies \vec{A} &= \frac{k\vec{C} + \vec{V}}{k+1}  
%\\
%\implies \vec{V} &= \frac{\brak{k+1}\vec{A} - k\vec{C}}{k}  
%\end{align}
%%
%for $k = 0.2$. \eqref{eq:tri_section_formula} is known as the {\em section formula}.
%%
%The python code for  Fig. \ref{fig:tri_sum_angle} is
%\begin{lstlisting}
%codes/triangle/tri_sum_angle.py
%\end{lstlisting}
%%
%and the equivalent latex-tikz code is
%%
%\begin{lstlisting}
%figs/triangle/tri_sum_angle.tex
%\end{lstlisting}
%\end{enumerate}
%\subsection{Baudhayana Theorem}
%Use Fig. \ref{fig:tri_baudh} for all problems in this section.
%\renewcommand{\theequation}{\theenumi}
%\begin{enumerate}[label=\arabic*.,ref=\thesubsection.\theenumi]
%\numberwithin{equation}{enumi}
%
%
%
%\item  Show that
%	\begin{equation}
%	\cos \theta = \sin \brak{90\degree - \theta}
%	\end{equation}
%
%
%\begin{figure}[!ht]
%	\begin{center}
%		\resizebox{\columnwidth}{!}{\input{./figs/triangle/tri_baudh.tex}}
%	\end{center}
%	\caption{Baudhayana Theorem}
%	\label{fig:tri_baudh}	
%\end{figure}
%
%
%\solution From Problem \ref{prob:tri_compl_angle} and  \eqref{eq:tri_trig_defs}
%%
%\begin{multline}
%\label{eq:tri_90-ang}
%\cos \angle BAC = \cos \alpha =	\cos \brak{90\degree-\theta} = \frac{c}{b} 
%\\
%= \sin \angle ABC = \sin \theta
%\end{multline}
%%
%\item
%Show that 
%%
%\begin{equation}
%\label{ch1_budh_basic}
%b = a \cos \theta + c \sin \theta
%\end{equation}
%%
%\solution We observe that
%%
%\begin{align}
%BD &= a \cos \theta \\
%AD &= c \cos\alpha = c \sin \theta \quad \brak{\text{From} \quad \eqref{eq:tri_90-ang}
%}
%\end{align}
%%
%Thus,
%\begin{equation}
%BD + AD = b = a \cos \theta + c \sin \theta
%\end{equation}
%\item
%From \eqref{ch1_budh_basic}, show that
%%
%\begin{equation}
%%
%\label{eq:tri_sin_cos_id}
%\sin ^2 \theta + \cos ^2 \theta = 1
%\end{equation}
%
%
%%
%\solution Dividing both sides of \eqref{ch1_budh_basic} by $b$, 
%\begin{align}
%1 &= \frac{a}{b}\cos\theta + \frac{c}{b}\sin\theta\\
%\Rightarrow &\sin ^2 \theta + \cos ^2 \theta = 1 \quad \brak{\text{from} \quad \eqref{eq:tri_trig_defs}}
%\end{align}
%
%\item
%	Using \eqref{ch1_budh_basic}, show that
%	\begin{equation}
%	\label{eq:tri_baudh}
%	c^2 = a^2 + b^2
%	\end{equation}
%	\eqref{eq:tri_baudh} is known as the Baudhayana theorem.  It is also known as the Pythagoras theorem.
%
%\solution From \eqref{ch1_budh_basic},
%\begin{align}
%c &= a\frac{a}{c} + b \frac{b}{c} \quad \brak{\text{from} \quad \eqref{eq:tri_trig_defs}}\\
%\Rightarrow c^2 &= a^2 + b^2
%\end{align}
%%
%%
%\item Draw Fig. \ref{fig:tri_baudh} for $a = 4, c =3$.
%\label{const:tri_baudh}
%%
%\\
%\solution Problem \ref{const:tri_right_angle} is used to draw $\triangle ABC$.
%%
%Using Problem \ref{prob:tri_polar},
%\begin{align}
%\vec{D} &= BD\myvec{\cos \alpha\\  \sin \alpha} 
%&= a \sin \theta \myvec{ \sin \theta \\ \cos \theta } 
%\label{eq:tri_baudh_foot}
%\end{align}
%%
%Using \eqref{eq:tri_baudh_foot}, the python code for  Fig. \ref{fig:tri_baudh} is
%\begin{lstlisting}
%codes/triangle/tri_baudh.py
%\end{lstlisting}
%%
%and the equivalent latex-tikz code is
%%
%\begin{lstlisting}
%figs/triangle/tri_baudh.tex
%\end{lstlisting}
%%
%\item Using 	\eqref{eq:tri_baudh}, for $a = 4, c = 3$,
%%
%\begin{align}
%b = \sqrt{a^2+c^2} = \sqrt{4^2+3^2} = 5
%\end{align}
%%
%\item For  point $\vec{D} = \myvec{d_1\\d_2}$, its {\em norm} is defined as
%%
%\begin{align}
%OD = d_1^2+d_2^2 = \norm{\vec{D}} \define \sqrt{\vec{D}^T\vec{D}}, 
%\label{eq:tri_norm_def}
%\end{align}
%%
%where 
%%
%\begin{align}
%\label{eq:tri_transpose_def}
% \vec{D}^T  \define \myvec{d_1 & d_2},
%\\
%\vec{D}^T\vec{D} \define \myvec{d_1 & d_2} \myvec{d_1 \\ d_2} = d_1^2+d_2^2
%\end{align}
%%
%\eqref{eq:tri_transpose_def} is the definition of {\em transpose}. $\vec{D}$ is defined to be a {\em column vector} and $\vec{D}^T$  is the corresponding {\em row vector} representing the same point.
%
%\item Also, it is easy to verify that
%%
%\begin{align}
%\label{eq:tri_norm_dist}
%AC \define  \norm{\vec{A}-\vec{C}} =  \norm{\myvec{4\\-3}} = \sqrt{3^2+4^2} = 5
%\end{align}
%%
%This is known as the {\em distance formula}.
%%
%\item Prove the distance formula in \eqref{eq:tri_norm_dist} using Baudhayana theorem.
%
%\end{enumerate}
%%\subsection{Area of a Triangle}
%%\renewcommand{\theequation}{\theenumi}
%%\begin{enumerate}[label=\arabic*.,ref=\thesubsection.\theenumi]
%%\numberwithin{equation}{enumi}
%%%
%%
%%
%%
%%\item
%%	The area of the rectangle $ACBD$ shown in Fig. \ref{fig:tri_rect} is defined as $ac$. Note that all the angles in the rectangle are $90\degree$
%%%	\label{fig:tri_rect}
%%
%%\begin{figure}[!ht]
%%	\begin{center}
%%		
%%		%\includegraphics[width=\columnwidth]{./figs/fig:tri_rect}
%%		%\vspace*{-10cm}
%%		\resizebox{\columnwidth}{!}{\input{./figs/triangle/tri_rect.tex}}
%%	\end{center}
%%	\caption{Area of a Right Triangle}
%%	\label{fig:tri_rect}	
%%\end{figure}
%%%
%%\item Draw Fig. \ref{fig:tri_rect} for $a = 4, c =3$.
%%\label{const:tri_rect}
%%\\
%%\solution Letting
%%%
%%\begin{align}
%%\vec{B} = \myvec{0 \\  0}, 
%%\vec{D} = \myvec{4 \\  3} 
%%\label{eq:tri_rect}
%%\end{align}
%%%
%%the python code for  Fig. \ref{fig:tri_rect} is
%%\begin{lstlisting}
%%codes/triangle/tri_rect.py
%%\end{lstlisting}
%%%
%%and the equivalent latex-tikz code is
%%%
%%\begin{lstlisting}
%%figs/triangle/tri_rect.tex
%%\end{lstlisting}
%%
%%\item
%%	The area of the two triangles constituting the rectangle is the same.
%%	\label{ch2_triang_eq}
%%
%%\item
%%	The area of the rectangle is the sum of the areas of the two triangles inside.
%%	\label{ch2_triang_sum}
%%
%%
%%\item
%%\label{prob:ch2_triang_area}
%%	Show that the area of $\Delta ABC$ is $\frac{ac}{2}$
%%
%%\begin{figure}[!ht]
%%	\begin{center}
%%		
%%		%\includegraphics[width=\columnwidth]{./figs/ch2_triang_ar}
%%		%\vspace*{-10cm}
%%		\resizebox{\columnwidth}{!}{\input{./figs/triangle/tri_sss.tex}}
%%	\end{center}
%%	\caption{Area of a Triangle}
%%	\label{fig:tri_sss}	
%%\end{figure}
%%
%%\solution From\eqref{ch2_triang_sum},
%%\begin{equation}
%%\label{ch2_triang_ar_1}
%%ar\brak{ABCD} = ar\brak{ACB} + ar\brak{ADB}
%%\end{equation}
%%Also from \eqref{ch2_triang_eq},
%%\begin{equation}
%%\label{ch2_triang_ar_2}
%%ar\brak{ACB} = ar\brak{ADB}
%%\end{equation}
%%From \eqref{ch2_triang_ar_1} and \eqref{ch2_triang_ar_2},
%%\begin{align}
%%2ar\brak{ACB} &= ar\brak{ABCD} = ac \brak{\text{from} \quad \eqref{fig:tri_rect}}
%%\\
%%\Rightarrow ar\brak{ACB} &= \frac{ac}{2}
%%\end{align}
%%
%%\item
%%	Show that the area of $\Delta ABC$ in Fig. 	\ref{fig:tri_sss}	is $\frac{1}{2}ah$.
%%
%%
%%\solution In Fig. \ref{fig:tri_sss},
%%\begin{align}
%%ar\brak{\Delta ADC} &= \frac{1}{2}hy \\
%%ar\brak{\Delta ADB} &= \frac{1}{2}hx 
%%\end{align}
%%Thus,
%%\begin{align}
%%ar\brak{\Delta ABC} &= ar\brak{\Delta ADC} + ar\brak{\Delta ADB} \\
%%&= \frac{1}{2}hy + \frac{1}{2}hx = \frac{1}{2}h\brak{x+y} \\
%%&= \frac{1}{2}ah
%%\end{align}
%%%
%%\item Draw Fig. \ref{fig:tri_sss} with $a=6$, $b=5$  and $c=4$.  
%%\label{const:tri_sss}
%%\\
%%\solution Let the vertices of  $\triangle ABC$ and $\vec{D}$ be 
%%\begin{align}
%%\label{eq:tri_basic}
%%\vec{A} = \myvec{p\\q}, \vec{B} = \myvec{0\\0}, \vec{C} = \myvec{a\\0}, \vec{D} = \myvec{p\\0}
%%\end{align}
%%%
%%
%%Then
%%\begin{align}
%%\label{eq:c_tricoord}
%%AB &= \norm{\vec{A}-\vec{B}}^2 = \norm{\vec{A}}^2  = c^2 \quad \because \vec{B} = \vec{0}
%%\\
%%\label{eq:a_tricoord}
%%BC &= \norm{\vec{C}-\vec{B}}^2 = \norm{\vec{C}}^2  = a^2
%%\\
%%AC &= \norm{\vec{A}-\vec{C}}^2 =    b^2
%%\label{eq:b_tricoord}
%%\end{align}
%%%
%%From \eqref{eq:b_tricoord},
%%\begin{align}
%%b^2 &=\norm{\vec{A}-\vec{C}}^2 = \norm{\vec{A}-\vec{C}}^T\norm{\vec{A}-\vec{C}}  
%%\\
%%&= \vec{A}^T\vec{A}+\vec{C}^T\vec{C}-\vec{A}^T\vec{C} - \vec{C}^T\vec{A} 
%%\\
%%&= \norm{\vec{A}}^2 + \norm{\vec{C}}^2 - 2\vec{A}^T\vec{C} \quad \brak{\because \vec{A}^T\vec{C} = \vec{C}^T\vec{A} } 
%%\label{eq:tri_const_norm_ac}
%%\\
%%&= a^2+c^2-2ap
%%\end{align}
%%%
%%yielding
%%\begin{align}
%%p&= \frac{a^2+c^2-b^2}{2a}
%%\end{align}
%%%
%%From \eqref{eq:c_tricoord}, 
%%\begin{align}
%%\norm{\vec{A}}^2 &= c^2 = p^2+q^2
%%\\
%%\implies q&= \pm \sqrt{c^2-p^2}
%%\end{align}
%%%
%%The python code for  Fig. \ref{fig:tri_sss} is
%%\begin{lstlisting}
%%codes/triangle/tri_sss.py
%%\end{lstlisting}
%%%
%%and the equivalent latex-tikz code is
%%%
%%\begin{lstlisting}
%%figs/triangle/tri_sss.tex
%%\end{lstlisting}
%%
%%\item
%%\label{prob:tri_area_sin}
%%	Show that the area of $\Delta ABC$ in Fig. 	\ref{fig:tri_sss}	is $\frac{1}{2}ab \sin C$.
%%
%%\solution We have
%%%
%%\begin{equation}
%%ar\brak{\Delta ABC} = \frac{1}{2}ah = \frac{1}{2}ab\sin C \quad \brak{\because \quad h = b \sin C}.
%%\end{equation}
%%%
%%\item
%%	Show that 
%%	\begin{equation}
%%	\frac{\sin A}{a} = \frac{\sin B}{b} = \frac{\sin C}{c}
%%	\end{equation}
%%
%%\solution Fig. \ref{fig:tri_sss} can be suitably modified to obtain 
%%\begin{equation}
%%ar\brak{\Delta ABC} = \frac{1}{2}ab\sin C = \frac{1}{s}bc\sin A = \frac{1}{2}ca\sin B
%%\end{equation}
%%Dividing the above by $abc$, we obtain
%%	\begin{equation}
%%\label{eq:tri_sin_form}
%%	\frac{\sin A}{a} = \frac{\sin B}{b} = \frac{\sin C}{c}
%%	\end{equation}
%%This is known as the sine formula.	
%%%
%%\item
%%In Fig. \ref{fig:tri_cosine_formula}, show that
%%%
%%\begin{equation}
%%\label{eq:tri_cos_form}
%%\cos A = \frac{b^2+c^2-a^2}{2bc}
%%\end{equation}
%%%
%%\
%%
%%\begin{figure}[!ht]
%%	\begin{center}
%%		
%%		%\includegraphics[width=\columnwidth]{./figs/ch2_triang_ar}
%%		%\vspace*{-10cm}
%%		\resizebox{\columnwidth}{!}{\input{./figs/triangle/tri_cosine_formula.tex}}
%%	\end{center}
%%	\caption{The cosine formula}
%%	\label{fig:tri_cosine_formula}	
%%\end{figure}
%%
%%\solution From the figure, the first of the following equations
%%%
%%\begin{align}
%%a &= b \cos C + c \cos B \\
%%b &= c \cos A + a \cos C \\
%%c &= b \cos A + a \cos B
%%\end{align}
%%%
%%is obvious and the other two can be similarly obtained.  The above equations can be expressed in matrix form as
%%%
%%\begin{equation}
%%\begin{pmatrix}
%%0 & c & b \\
%%c & 0 & a \\
%%b & a & 0
%%\end{pmatrix}
%%\begin{pmatrix}
%%\cos A \\
%%\cos B \\
%%\cos C
%%\end{pmatrix}
%%= 
%%\begin{pmatrix}
%%a\\
%%b\\
%%c
%%\end{pmatrix}
%%\end{equation}
%%%
%%Using the properties of determinants,
%%%
%%\begin{align}
%%\cos A &= \frac{
%%\begin{vmatrix}
%%a & c & b \\
%%b & 0 & a \\
%%c & a & 0
%%\end{vmatrix}
%%	}
%%	{
%%\begin{vmatrix}
%%0 & c & b \\
%%c & 0 & a \\
%%b & a & 0
%%\end{vmatrix}
%%	}
%%	=\frac{ab^2 + ac^2 - a^3}{abc + abc} 
%%\\
%%&= \frac{b^2 + c^2 - a^2}{2abc}
%%\end{align}
%%%
%%\item Find Hero's formula for the area of a triangle.
%%\\
%%\solution 
%%%In Fig. \ref{fig:rt_triangle}, from Baudhayana's theorem, 
%%%\begin{align}
%%%\label{eq:tri_geo_baudh}
%%%b^2 = a^2+c^2 &
%%%\\
%%%=b^2\cos^2C+b^2\sin^2C &
%%%\\
%%%\implies \cos^2C+\sin^2C &= 1
%%%\end{align}
%%%
%%%In Fig. \ref{fig:tri_const_ex_cos_form}, 
%%From \eqref{prob:tri_area_sin}, the area of $\triangle ABC$ is 
%%{\footnotesize
%%\begin{align}
%%\label{eq:tri_geo_area_sin_form}
%% \frac{1}{2}ab\sin C
%%%\\
%%&=\frac{1}{2}ab\sqrt{1-\cos^2C} 
%%\quad \brak{\text{from } \eqref{eq:tri_sin_cos_id}
%%%\eqref{eq:tri_geo_baudh}
%%}
%%\\
%%&=\frac{1}{2}ab\sqrt{1-\brak{\frac{a^2+b^2-c^2}{2ab}}^2} \brak{\text{from } \eqref{eq:tri_cos_form}
%%}
%%\\
%%&=\frac{1}{4}\sqrt{\brak{2ab}^2-\brak{a^2+b^2-c^2}}
%%\\
%%&=\frac{1}{4}\sqrt{\brak{2ab+a^2+b^2-c^2}\brak{2ab-a^2-b^2+c^2}}
%%\\
%%&= \frac{1}{4}\sqrt{\cbrak{\brak{a+b}^2-c^2}\cbrak{c^2-\brak{a-b}^2}}
%%\\
%%&= \frac{1}{4}\sqrt{\brak{a+b+c}\brak{a+b-c}\brak{a+c-b}\brak{b+c-a}}
%%\label{eq:tri_ex_hero_temp}
%%\end{align}
%%}
%%Substituting 
%%%
%%\begin{align}
%%s=\frac{a+b+c}{2}
%%\end{align}
%%%
%%in \eqref{eq:tri_ex_hero_temp}, the area of $\triangle ABC$ is 
%%%
%%\begin{align}
%%\label{eq:tri_hero}
%%\sqrt{s\brak{s-a}\brak{s-b}\brak{s-c}}
%%\end{align}
%%%
%%This is known as Hero's formula.
%%\end{enumerate}
%%
%
