\renewcommand{\theequation}{\theenumi}
\begin{enumerate}[label=\arabic*.,ref=\thesubsection.\theenumi]
\numberwithin{equation}{enumi}
\item The equation of a circle is 
\begin{align}
\label{eq:circ_norm}
\norm{\vec{x}-\vec{c}} = r
\end{align}
%
where $\vec{c}$ is the centre and $r$ is the radius.
\item By expanding \eqref{eq:circ_norm}, the equation of a circle can also be expressed as
%
\numberwithin{equation}{enumi}
\begin{align}
\norm{\vec{x}-\vec{c}}^2 = r^2&
\\
\implies \vec{x}^T\vec{x}-2\vec{c}^T\vec{x} + \vec{c}^T\vec{c}-r^2 = 0
\label{eq:circ_quad}
\end{align}
\item Find the equation of the {\em circumcircle} of  $\triangle ABC$ in Fig. \ref{fig:ccircle}.
\\
\solution Let $\vec{O}$ be the centre and $R$ the radius. From \eqref{eq:circ_quad},
\begin{align}
%\label{eq:circ_quad}
\norm{\vec{A}-\vec{O}}^2 = \norm{\vec{B}-\vec{O}}^2 = \norm{\vec{C}-\vec{O}}^2 &= R^2
\\
\implies \norm{\vec{A}-\vec{O}}^2 - \norm{\vec{B}-\vec{O}}^2 &=0
\end{align}
which can be simplified to obtain
\begin{align}
\label{eq:defs_ccircle_c1}
\brak{\vec{A}-\vec{B}}^T\vec{O}=\frac{\norm{\vec{A}}^2 - \norm{\vec{B}}^2}{2}& \quad \text{and}
\\
\brak{\vec{A}-\vec{C}}^T\vec{O}=\frac{\norm{\vec{A}}^2 - \norm{\vec{C}}^2}{2}& 
\label{eq:defs_ccircle_c2}
\end{align}
%
Solving the two yields $\vec{O}$, which can then be used to obtain $R$.
\item Given
$OD \perp BC$ as in Fig. \ref{fig:ccircle}.  Show that 
\begin{align}
\vec{D}=\frac{\vec{B}+\vec{C}}{2}
\end{align}
%
\begin{figure}[!ht]
	\begin{center}
		
		%\includegraphics[width=\columnwidth]{./figs/ch3_angle_bisector}
		%\vspace*{-10cm}
		\resizebox{\columnwidth}{!}{\input{./circle/figs/ccircle.tex}}
	\end{center}
	\caption{Circumcircle.}
	\label{fig:ccircle}	
\end{figure}


\solution From \eqref{eq:circ_norm}
\begin{align}
\norm{\vec{B}-\vec{O}}^2=\norm{\vec{C}-\vec{O}}^2=R^2
\\
 \implies \brak{\vec{B}-\vec{O}}^T\brak{\vec{B}-\vec{O}} = 
\brak{\vec{C}-\vec{O}}^T\brak{\vec{C}-\vec{O}} 
\\
 \implies \brak{\vec{B}-\vec{C}}^T\brak{\frac{\vec{B}+\vec{C}}{2} - 
\vec{O}}  = 0
\label{eq:circle_mid}
\end{align}
after simplification. Since $OD \perp BC$,
\begin{align}
\brak{\vec{B}-\vec{C}}^T\brak{\vec{D}-\vec{O}} = 0 
\label{eq:circle_D}
\end{align}
Since $D$ and $\frac{\vec{B}+\vec{C}}{2}$ lie on $BC$, using 
\eqref{eq:line_ab},
\begin{align}
\label{eq:circle_mid_D1}
\frac{\vec{B}+\vec{C}}{2}
&= \vec{B}+ \lambda_1\brak{\vec{B}-\vec{C}}
\\
\vec{D}
&= \vec{B}+ \lambda_2\brak{\vec{B}-\vec{C}}
\label{eq:circle_mid_D2}
\end{align}
Multiplying \eqref{eq:circle_mid_D1} and \eqref{eq:circle_mid_D2} with 
$\brak{\vec{B}-\vec{C}}^T$ and subtracting, $\lambda_1=\lambda_2$
%
\begin{align}
\implies \vec{D} = \frac{\vec{B}+\vec{C}}{2}
\label{eq:circle_bisect}
\end{align}
%
\item Let  $\vec{D}$ be the mid point of $BC$.  Show that $OD \perp BC$.
%
\item The {\em incircle} with centre $\vec{I}$ and radius $r$ in Fig.\ref{fig:ang_bisect}	
 is inside 
$\triangle ABC$ and touches $AB, BC$ 
and $CA$ at $\vec{W}, \vec{U}$ and $\vec{V}$ respectively. $AB, BC$ and 
$CA$ are known as {\em tangents} to the circle.
\begin{figure}[!ht]
	\begin{center}
		
		%\includegraphics[width=\columnwidth]{./figs/ch3_angle_bisector}
		%\vspace*{-10cm}
		\resizebox{\columnwidth}{!}{\input{./circle/figs/ang_bisect.tex}}
	\end{center}
	\caption{Tangent and incircle.}
	\label{fig:ang_bisect}	
\end{figure}


\item Show that $IU \perp BC$.
%\begin{figure}[!h]
%\centering
%\resizebox {\columnwidth} {!} {
%\input{./figs/derivative.tex}
%}
%\caption{Notion of the derivative.}
%\label{fig:derivative}
%\end{figure}
\\
\solution Let $\vec{x}_1,\vec{x}_2$ be two points on the circle such that 
$x_1x_2 \parallel BC$. Then
%
\begin{align}
\norm{\vec{x}_1-\vec{I}}^2- 
\norm{\vec{x}_2-\vec{I}}^2 &= 0 
\\
\implies 
\brak{\vec{x}_1-\vec{x}_2}^T\brak{\frac{\vec{x}_1+\vec{x}_2}{2}-\vec{I}} &= 
0 
\\
\implies 
\brak{\vec{B}-\vec{C}}^T\brak{\frac{\vec{x}_1+\vec{x}_2}{2}-\vec{I}} &= 
0 
%\label{eq:circle_bisect}
\end{align}
%
For $\vec{x}_1=\vec{x}_2=\vec{U}$, $x_1x_2$ merges into $BC$ and the above 
equation becomes 
%
\begin{align}
\brak{\vec{B}-\vec{C}}^T\brak{\vec{U}-\vec{I}} = 
0 
\implies OD \perp BC
%\label{eq:circle_bisect}
\end{align}
%
\item Give an alternative proof for the above.
\\
\solution Let 
\begin{align}
\vec{B} & = \mbf{0}
\\
\vec{U} &= \lambda \vec{m}
\end{align}
Then
\begin{align}
\norm{\vec{U} - \vec{I}}^2 = r^2 &
\\
\implies \lambda^2\norm{\vec{m}}^2 - 2\lambda\vec{m}^T\vec{I} + \norm{\vec{I}}^2 &= r^2 
\end{align}
Since the above equation has a single root,
\begin{align}
\lambda = \frac{\vec{m}^T\vec{I}}{\norm{\vec{m}}^2}
\label{eq:incircle_lam}
\end{align}
%
Thus, 
\begin{align}
\brak{\vec{U} - \vec{B}}^T\brak{\vec{U} - \vec{I}}
&= \brak{\lambda\vec{m}}^T
\brak{\lambda\vec{m}-\vec{I}}
\\
&=\lambda^2\norm{\vec{m}}^2-\lambda\vec{m}^T\vec{I}
\\
&= \mbf{O} \text{ (from \ref{eq:incircle_lam})}.
\\
\implies & OD \perp BC
\end{align}
\item Find the equation of the tangent at $\vec{U}$.
\\
\solution The equation of the tangent is given by 
\begin{align}
\brak{\vec{I}-\vec{U}}^T\brak{\vec{x}-\vec{U}}=0
%\label{eq:circle_bisect}
\end{align}
%
\item The direction vector of {\em normal to the circle}  in \eqref{eq:circ_quad} at point $\vec{U}$ is
\begin{align}
\label{eq:circ_normal}
\vec{n} = \vec{U}-\vec{I}
\end{align}
%
%where $k$ is a constant.
\item Find an expression for $r$ if $\vec{I}$ is known.
\\
\solution Let $\vec{n}$ be the normal vector of $BC$.  The equation for $BC$ is then given by
\begin{align}
\vec{n}^T\brak{\vec{x}-\vec{B}} &= 0
\\
\implies \vec{n}^T\brak{\vec{U}-\vec{B}} &= 0
\label{eq:incirc_ub}
\end{align}
since $\vec{U}$ lies on $BC$.
Since $IU \perp BC$, 
\begin{align}
\label{eq:incirc_iu}
\vec{I}&=\vec{U}+\lambda\vec{n}
\\
\implies \vec{I}-\vec{U}&=\lambda\vec{n}
\\
\text{or}\quad r=\norm{\vec{I}-\vec{U}}&=\abs{\lambda}\norm{\vec{n}}
\label{eq:incirc_r}
\end{align}
From \eqref{eq:incirc_ub} and \eqref{eq:incirc_iu}
\begin{align}
\vec{n}^T\vec{I}&=\vec{n}^T\vec{B}+\lambda\vec{n}^T\vec{n}
\\
\implies \vec{n}^T\brak{\vec{I}-\vec{B}}&=\lambda\norm{\vec{n}}^2
\\
\implies r = \abs{\lambda}\norm{\vec{n}}&=\frac{\abs{\vec{n}^T\brak{\vec{I}-\vec{B}}}}{\norm{\vec{n}}}
\end{align}
from \eqref{eq:incirc_r}.  Letting 
\begin{align}
\norm{\vec{n}_1}&= \frac{\vec{n}}{\norm{\vec{n}}},
\\
r &= \abs{\vec{n}_1^T\brak{\vec{I}-\vec{B}}}
\label{eq:incirc_rad}
\end{align}
\item Find $\vec{I}$.
\\
\solution Since $r = IU = IV = IW$, from \eqref{eq:incirc_rad},
\begin{align}
\abs{\vec{n}_1^T\brak{\vec{I}-\vec{B}}} = \abs{\vec{n}_2^T\brak{\vec{I}-\vec{C}}} = 
\abs{\vec{n}_3^T\brak{\vec{I}-\vec{A}}}
\label{eq:incirc_radeq}
\end{align}
%
where $\vec{n}_2, \vec{n}_3$ are unit normals of $CA, AB$ respectively.  \eqref{eq:incirc_radeq} can be 
expressed as 
\begin{align}
\vec{n}_1^T\brak{\vec{I}-\vec{B}} &= k_1\vec{n}_2^T\brak{\vec{I}-\vec{C}} 
\\
\vec{n}_2^T\brak{\vec{I}-\vec{C}} &= k_2\vec{n}_3^T\brak{\vec{I}-\vec{A}}
\label{eq:incirc_k1k2}
\end{align}
%
where $k_1,k_2 = \pm 1$. The above equations can be expressed as the matrix equation
\begin{align}
\myvec{\vec{n}_1-k_1\vec{n}_2 & \vec{n}_2 - k_2\vec{n}_3}^T\vec{I} &= 
\myvec{\vec{n}_1^T\vec{B}-k_1\vec{n}_2^T\vec{C} \\ \vec{n}_2^T \vec{C} - k_2\vec{n}_3^T\vec{A}}
\label{eq:incirc_k1k2fin}
\end{align}
\item Show that $\vec{I}$ lies inside $\triangle ABC$ for $k_1=k_2=1$
%\label{eq:line_dist_pt}
\item Let $a = BC, b = CA$, $ c= AB$, $x = BU=BW$, $y = CU=CV$, $z = AV=AW$. Find $\vec{U}$.
\\
\solution It is easy to verify that 
\begin{align}
\label{eq:incircle_mat}
\myvec{1 & 1 & 0\\0 & 1 & 1\\1 & 0 & 1}\myvec{x\\y\\z} = \myvec{a\\b\\c}
\end{align}
%
which can be used to obtain $x$ and $y$.
Using the section formula, 
\begin{align}
\vec{U} = \frac{x\vec{B}+\vec{A}}{x+y}
\end{align}

\item Show that the angle in a semi-circle is a right angle.
\begin{figure}[!h]
\centering
\resizebox {\columnwidth} {!} {
\input{./circle/figs/semi_circle.tex}
}
\caption{Angle in a semi-circle.}
\label{fig:ch2_line}
\end{figure}
\\
\solution Let 
\begin{align}
\vec{O} = 0
\end{align}
From the given information,
\begin{align}
\label{eq:semi_circ_pt}
\norm{\vec{A}}^2 = \norm{\vec{B}}^2 = \norm{\vec{C}}^2 = r^2
\\
\norm{\vec{B}-\vec{C}}^2 =  \brak{2r}^2
\\
\vec{B} + \vec{C} = 0
\label{eq:semcirc_mid}
\end{align}
%
where $r$ is the radius of the circle. Thus,
\begin{multline}
\norm{\vec{A}-\vec{B}}^2 + \norm{\vec{A}-\vec{C}}^2 = 
2\norm{\vec{A}}^2 + \norm{\vec{B}}^2 + \norm{\vec{C}}^2
\\
-2\vec{A}^T\brak{\vec{B}+\vec{C}}
%\\
%\norm{\vec{B}-\vec{C}}^2 =  \brak{2r}^2
%\\
%\vec{B} + \vec{C} = 0
\end{multline}
From \eqref{eq:semcirc_mid} and \eqref{eq:semi_circ_pt},
\begin{multline}
\norm{\vec{A}-\vec{B}}^2 + \norm{\vec{A}-\vec{C}}^2 = 4r^2 = \norm{\vec{B}-\vec{C}}^2 
%\\
%\norm{\vec{B}-\vec{C}}^2 =  \brak{2r}^2
%\\
%\vec{B} + \vec{C} = 0
\end{multline}
Thus, using Baudhayana's theorem, $\triangle ABC$ is right angled.
\item 	Show that $PA.PB = PC^2$, where $PC$ is the tangent to the circle in Fig. \ref{fig:tangent_secant}.

	\begin{figure}[!hb]
		\begin{center}
			
			%\includegraphics[width=\columnwidth]{./figs/ch4_tangent_prod}
			%\vspace*{-10cm}
			\resizebox{\columnwidth}{!}{\input{./circle/figs/tangent_secant.tex}}
		\end{center}
		\caption{$PA.PB = PC^2$.}
		\label{fig:tangent_secant}	
	\end{figure}
\solution Let $\vec{P} = \mbf{0}$.  Then, we have the following equations
\begin{align}
\label{eq:tan_sec_AB}
PA.PB &= \lambda \norm{\vec{A}}^2 \quad \because (\vec{B} = \lambda \vec{A})
\\
\norm{\vec{A}-\vec{O}}^2 &= \norm{\vec{B}-\vec{O}}^2 = \norm{\vec{C}-\vec{O}}^2 = r^2
\\
\norm{\vec{O}}^2-\norm{\vec{C}}^2 &=  r^2 \quad \triangle PCO\text{ is 
right angled}
\label{eq:tan_sec_boudh}
\end{align}
$\because$
\begin{align}
%\label{eq:tan_sec_AB}
%PA.PB &= \lambda \norm{\vec{A}}^2 \quad \because (\vec{B} = \lambda 
%\vec{A})
%\\
\norm{\vec{B}-\vec{O}}^2-\norm{\vec{A}-\vec{O}}^2   &=0,
\\
\brak{\lambda^2-1}\norm{\vec{A}}^2 - 2 \brak{\lambda-1}\vec{A}^T\vec{O} &= 
0
\\
\implies PA.PB = \lambda\norm{\vec{A}}^2 =  2 
\vec{A}^T\vec{O}-\norm{\vec{A}}^2 &
%\norm{\vec{C}-\vec{O}}^2 = r^2
%\\
%\norm{\vec{O}}^2-\norm{\vec{C}}^2 &=  r^2 \quad \triangle PCO\text{ is 
%right angled}
%\label{eq:tan_sec_boudh}
\label{eq:tan_sec_first}
\end{align}
after substituting from \eqref{eq:tan_sec_AB} and simplifying. From 
\eqref{eq:tan_sec_boudh},
\begin{align}
\norm{\vec{A}-\vec{O}}^2 = \norm{\vec{O}}^2-\norm{\vec{C}}^2  &= r^2
\\
\implies 2 \vec{A}^T\vec{O}-\norm{\vec{A}}^2   = \norm{\vec{C}}^2 = PC^2&
\label{eq:tan_sec_second}
\end{align}
From \eqref{eq:tan_sec_first} and \eqref{eq:tan_sec_second},
\begin{align}
PA.PB = PC^2
\end{align}

\item In Fig. \ref{fig:chords} show that $PA.PB = PC.PD$.
\begin{figure}[!ht]
	\begin{center}
		
		%\includegraphics[width=\columnwidth]{./figs/ch3_angle_bisector}
		%\vspace*{-10cm}
		\resizebox{\columnwidth}{!}{\input{./circle/figs/chords.tex}}
	\end{center}
	\caption{Chords of a circle}
	\label{fig:chords}	
\end{figure}
\\
\solution Let $\vec{P} = \mbf{0}$.  We then have the following equations
\begin{align}
\begin{split}
\vec{B} &= k_1 \vec{A}, k_1 = \frac{PB}{PA}
\\
\vec{D} &= k_2 \vec{C}, k_2 = \frac{PD}{PC}
\end{split}
\label{eq:chords_ratio}
\\
\begin{split}
\norm{\vec{A}-\vec{O}}^2 &= \norm{\vec{B}-\vec{O}}^2 
\\
= \norm{\vec{C}-\vec{O}}^2 &= \norm{\vec{D}-\vec{O}}^2 = r^2
\end{split}
\label{eq:chords_points}
\end{align}
%
where $r$ is the radius of the circle and $\vec{O}$ is the centre. From \eqref{eq:chords_points},
\begin{align}
&\norm{\vec{A}-\vec{O}}^2 = \norm{\vec{B}-\vec{O}}^2
\\
\implies &\norm{\vec{A}-\vec{O}}^2 = \norm{k\vec{A}-\vec{O}}^2 \quad(\text{from \eqref{eq:chords_ratio}})
\end{align}
%
which can be simplified to obtain
\begin{align}
k_1\norm{\vec{A}}^2 = 2\vec{A}^T\vec{O}-\norm{\vec{A}}^2
\label{eq:chords_Anorm}
\end{align}
Similarly,
\begin{align}
k_2\norm{\vec{C}}^2 = 2\vec{C}^T\vec{O}-\norm{\vec{C}}^2
\label{eq:chords_Cnorm}
\end{align}
%
From \eqref{eq:chords_points}, we also obtain
\begin{align}
\norm{\vec{A}-\vec{O}}^2 
= \norm{\vec{C}-\vec{O}}^2 
\\
\implies 2\vec{A}^T\vec{O}-\norm{\vec{A}}^2 = 2\vec{C}^T\vec{O}-\norm{\vec{C}}^2
\label{eq:chords_ACnorm}
\end{align}
%
after simplification. Using this result in \eqref{eq:chords_Anorm} and \eqref{eq:chords_Cnorm},
\begin{align}
k_1\norm{\vec{A}}^2 = k_2\norm{\vec{C}}^2
\\
\implies \norm{\vec{A}}\, \norm{\vec{B}}=\norm{\vec{C}}\,\norm{\vec{D}}
\end{align}
which completes the proof.

\item (Pole and Polar:) The polar of a point $\vec{x}$ with respect to the curve
\begin{align}
\label{eq:quad_form_polar}
\vec{x}^T\vec{V}\vec{x}+2\vec{u}^T\vec{x}+f=0
\end{align}
is the line
\begin{align}
\label{eq:polar}
\vec{n}^T\vec{x} = c
\end{align}
%
where
\begin{align}
\myvec{\vec{n}^T\\ - c}=
\myvec{
\vec{V}&\vec{u}
\\
\vec{u}^T&f
}
\myvec{\vec{x}\\1}
\end{align}
%
The pole of the line  in \eqref{eq:polar} is obtained as $\frac{1}{x_3}\myvec{x_1\\x_2}$, where
\begin{align}
\myvec{x_1 \\ x_2\\x_3}
=\myvec{
\vec{V}&\vec{u}
\\
\vec{u}^T&f
}^{-1}
\myvec{\vec{n}^T\\ - c}
\end{align}
\item $\vec{x}_1$ and $\vec{x}_2$ are said to be conjugate points for \eqref{eq:quad_form_polar} if $\vec{x}_2$ lies on the polar of $\vec{x}_1$ and vice-versa.  A similar definition holds for conjugate lines as well.
\item Let $\vec{p}$ be a point of intersection of two circles with centres $\vec{c}_1$ and $\vec{c}_2$.  The circles are said to be orthogonal if their tangents at $\vec{p}$ are perpendicular to each other.  Show that if $r_1$ and $r_2$ are their respective radii, 
\begin{align}
\label{eq:circ_orth}
\norm{\vec{c_1}-\vec{c}_2}^2 = r_1^2+r_2^2 
\end{align}
\item Show that the length of the tangent from a point $\vec{p}$ to the circle 
\begin{align}
\label{eq:circ_quad_len}
\vec{x}^T\vec{x}-2\vec{c}^T\vec{x} + f = 0
\end{align}
%
is 
\begin{align}
\label{eq:circ_tang_len}
\vec{p}^T\vec{p}-2\vec{c}^T\vec{p} + f 
\end{align}
This length is also known as the {\em power} of the point $\vec{p}$ with respect to the circle.
\item  The {\em radical axis} of the circles 
\begin{align}
%\label{eq:circs_two}
\vec{x}^T\vec{x}-2\vec{c}_1^T\vec{x} + f_1 = 0
\\
\vec{x}^T\vec{x}-2\vec{c}_2^T\vec{x} + f_2 = 0
\end{align}
%
is the locus of the points from which lengths of the tangents to the circles are equal.  From \eqref{eq:circs_two}, this locus is
\begin{align}
\vec{x}^T\vec{x}-2\vec{c}_1^T\vec{x} + f_1 -
%\nonumber \\
\vec{x}^T\vec{x}-2\vec{c}_2^T\vec{x} + f_2 = 0
\\
\implies 2\brak{\vec{c}_1-\vec{c}_2}^T\vec{x} + f_2 - f_1 = 0
\label{eq:circs_rad_axis}
\end{align}
\item Show that the radical axis of the circles is perpendicular to the line joining their centres.\item {\em Coaxal circles} have the same radical axis.
\item Obtain a family of coaxal circles from \label{eq:circs_two} and find their {\em limit points}.
\\
\solution The family of circles is obtained as
\begin{align}
\label{eq:circs_coaxal_family}
\vec{x}^T\vec{x}-2\brak{\vec{c}_1 +\lambda\vec{c}_2}^T\vec{x} + f_1 +\lambda f_2= 0
\end{align}
%
The limit points are the centres of those circles whose radii are 0. From \eqref{eq:circs_coaxal_family} and \eqref{eq:circ_quad},
this results in
\begin{align}
%\label{eq:circs_coaxal_family}
f_1 +\lambda f_2 =  \brak{\vec{c}_1 +\lambda\vec{c}_2}^T\brak{\vec{c}_1 +\lambda\vec{c}_2} &
\\
\implies \lambda^2 \norm{\vec{c}_2}^2 + \lambda \brak{2\vec{c}_1^T\vec{c}_2-f_2} + \norm{\vec{c}_1}^2-f_1 = 0&
\end{align}
Solving for $\lambda$, the limit points are given by  
\begin{align}
\vec{c}_1+\lambda\vec{c}_2
\end{align}
\end{enumerate}


